theories/calling_convention.v
@@ -10,7 +10,7 @@ Definition c_call `{!islaG Σ} `{!threadG} (stack_size : Z) (P : list valu → b
   ∃ (sp ret : bv 64),
   reg_col sys_regs ∗
   reg_col CNVZ_regs ∗
-  reg_col ((λ r, (RegColDirect r, None)) <$> tmp_registers) ∗
+  reg_col ((λ r, (KeyReg r, None)) <$> tmp_registers) ∗
   "R0" ↦ᵣ: λ r0, "R1" ↦ᵣ: λ r1, "R2" ↦ᵣ: λ r2, "R3" ↦ᵣ: λ r3, "R4" ↦ᵣ: λ r4, "R5" ↦ᵣ: λ r5,
   "R6" ↦ᵣ: λ r6, "R7" ↦ᵣ: λ r7, "R8" ↦ᵣ: λ r8, "R19" ↦ᵣ: λ r19, "R20" ↦ᵣ: λ r20, "R21" ↦ᵣ: λ r21,
   "R22" ↦ᵣ: λ r22, "R23" ↦ᵣ: λ r23, "R24" ↦ᵣ: λ r24, "R25" ↦ᵣ: λ r25, "R26" ↦ᵣ: λ r26, "R27" ↦ᵣ: λ r27,
@@ -23,8 +23,8 @@ Definition c_call `{!islaG Σ} `{!threadG} (stack_size : Z) (P : list valu → b
   instr_pre (bv_unsigned ret) (
       reg_col sys_regs ∗
       reg_col CNVZ_regs ∗
-      reg_col ((λ r, (RegColDirect r, None)) <$> ["R0"; "R1"; "R2"; "R3"; "R4"; "R5"; "R6"; "R7"]) ∗
-      reg_col ((λ r, (RegColDirect r, None)) <$> tmp_registers) ∗
+      reg_col ((λ r, (KeyReg r, None)) <$> ["R0"; "R1"; "R2"; "R3"; "R4"; "R5"; "R6"; "R7"]) ∗
+      reg_col ((λ r, (KeyReg r, None)) <$> tmp_registers) ∗
       "R0" ↦ᵣ: λ r0', "R1" ↦ᵣ: λ r1', "R2" ↦ᵣ: λ r2', "R3" ↦ᵣ: λ r3', "R4" ↦ᵣ: λ r4',
       "R5" ↦ᵣ: λ r5', "R6" ↦ᵣ: λ r6', "R7" ↦ᵣ: λ r7', "R8" ↦ᵣ: λ r8',
       "R19" ↦ᵣ r19 ∗ "R20" ↦ᵣ r20 ∗ "R21" ↦ᵣ r21 ∗ "R22" ↦ᵣ r22 ∗ "R23" ↦ᵣ r23 ∗ "R24" ↦ᵣ r24 ∗
